almost finished the while language semantics && proofs

while-program-infoflow/WhileProgram.dfy
@@ -85,6 +85,12 @@ module WhileProgram{
     ensures s.Keys == s'.Keys
     ensures typeOK(s') && VariablesInCmd(c') <= s'.Keys
     {}
+    predicate EmptyCmd(c: Cmd)
+    {
+        match c
+        case Skip => true
+        case _ => false
+    }
 
     // Next we define how a program terminates within n steps of transitions
     predicate Terminates(c: Cmd, s: MState, s': MState, n: int)
@@ -93,12 +99,143 @@ module WhileProgram{
     decreases n
     {
         match c {
-            case Skip => s == s' 
+            case Skip => s == s' && n == 0
             case _ => 
                 var (s1, c1) := TransitionSmallStep(s, c); 
                 TransitionSmallStepTypeOK(s, c, s1, c1);
+                // assert !EmptyCmd(c);
                 n >= 1 && Terminates(c1, s1, s', n-1)
         }
     }
+    // One step termination: after a small step, the remaining program terminates
+    lemma {:induction false} SmallStepTermination(s1: MState, s2: MState, c: Cmd, k: int) returns (s': MState, c': Cmd)
+    requires typeOK(s1) && typeOK(s2) && k >= 0
+    requires VariablesInCmd(c) <= s1.Keys == s2.Keys
+    requires Terminates(c, s1, s2, k)
+    requires !EmptyCmd(c)
+    ensures typeOK(s')
+    ensures (s', c') == TransitionSmallStep(s1, c) 
+    ensures VariablesInCmd(c') <= s'.Keys == s2.Keys
+    ensures Terminates(c', s', s2, k-1)
+    {
+        match c {
+            case Skip => 
+                assert false;
+            case Assn(x, e) => // assignment
+                s', c' := s1[x:= Evaluate(s1, e)], Skip;
+                assert typeOK(s');
+                assert VariablesInCmd(c') <= s'.Keys == s2.Keys;
+                assert k >= 1;
+                assert Terminates(c', s', s2, k-1); assert s2 == s';
+            case If(e, c1, c2) => // if-then-else
+                var res := Evaluate(s1, e);
+                if (res != 0){
+                    s', c' := s1, c1;
+                } else {
+                    s', c' := s1, c2;
+                }
+                assert typeOK(s');
+                assert k >= 1;
+            case While(e, c1) => // while-loop
+                var res := Evaluate(s1, e);
+                if (res != 0){
+                    s', c' := s1, Seq(c1, c);
+                } else {
+                    s', c' := s1, Skip;
+                }
+                assert typeOK(s');
+                assert k >= 1;
+            case Seq(c1, c2) => // sequential composition
+                match c1 {
+                    case Skip => 
+                        var p := TransitionSmallStep(s1, c2);
+                        s', c' := p.0, p.1;
+                        TransitionSmallStepTypeOK(s1, c, s', c');
+                        assert typeOK(s');
+                        assert k >= 1;
+                    case _ => 
+                        var (s3, c3) := TransitionSmallStep(s1, c1); 
+                        s', c' := s3, Seq(c3, c2);
+                        TransitionSmallStepTypeOK(s1, c, s', c');
+                        assert typeOK(s');
+                        assert k >= 1;
+                }
+        }
+        assert Terminates(c', s', s2, k-1);  
+        assert VariablesInCmd(c') <= s'.Keys == s2.Keys;
+        assert Terminates(c', s', s2, k-1);
+    }
+    // The complement of the above lemma, to prove later ...
+    lemma {:axiom} SkipTermination(s1: MState, s2: MState, c: Cmd, k: int)
+    requires typeOK(s1) && typeOK(s2) && k >= 0
+    requires VariablesInCmd(c) <= s1.Keys == s2.Keys
+    requires Terminates(Seq(Skip, c), s1, s2, k)
+    ensures Terminates(c, s1, s2, k)
+    // {}
 
+    // Multiple step termination for sequential composition
+    lemma {:induction false} Sequencing(s1: MState, s2: MState, c1: Cmd, c2: Cmd, k: int) returns (s': MState, k': int)
+    requires typeOK(s1) && typeOK(s2) && k >= 0
+    requires VariablesInCmd(c1) <= s1.Keys == s2.Keys
+    requires VariablesInCmd(c2) <= s1.Keys == s2.Keys
+    requires Terminates(Seq(c1, c2), s1, s2, k)
+    // requires !EmptyCmd(c1)
+    ensures typeOK(s') 
+    ensures k' >= 0 && k - k' >= 0 
+    ensures VariablesInCmd(c1) <= s1.Keys == s2.Keys == s'.Keys
+    ensures VariablesInCmd(c2) <= s1.Keys == s2.Keys == s'.Keys
+    ensures Terminates(c1, s1, s', k')
+    ensures Terminates(c2, s', s2, k - k')
+    decreases k, c1, c2
+    {
+        if (EmptyCmd(c1)){ // c1 == Skip // the base case
+            s' := s1; 
+            k' := 0;
+            assert typeOK(s');
+            SkipTermination(s1, s2, c2, k);
+            assert Terminates(c1, s1, s', k');
+            assert Terminates(c2, s', s2, k - k');
+        } else {
+            // need to consider a number of cases for c1
+            match c1 {
+                case Seq(c3, c4) => // sequential composition
+                    // if (EmptyCmd(c3) && EmptyCmd(c4)){ // Seq(Skip, Skip) => Skip 
+                    //     s' := s1; 
+                    //     k' := 1;
+                    //     assert Terminates(c1, s1, s', k');
+                    //     assert Terminates(c2, s', s2, k - k');
+                    // } // the above case is covered by the following case
+                    if (EmptyCmd(c3)) {
+                        var (s3, c5) := TransitionSmallStep(s1, c4);
+                        assert (s3, Seq(c5, c2)) == TransitionSmallStep(s1, Seq(c1, c2));
+                        TransitionSmallStepTypeOK(s1, Seq(c1,c2), s3, Seq(c5,c2));
+                        assert Terminates(Seq(c5, c2), s3, s2, k-1);
+                        assert typeOK(s3);
+                        var s4, k2 := Sequencing(s3, s2, c5, c2, k-1);
+                        s', k' := s4, k2+1;
+                        assert Terminates(c2, s', s2, k-k');
+                        assert Terminates(c1, s1, s', k');
+                    } else {
+                        var (s3, c5) := TransitionSmallStep(s1, c3); 
+                        assert (s3, Seq(Seq(c5, c4), c2)) == TransitionSmallStep(s1, Seq(c1, c2));
+                        TransitionSmallStepTypeOK(s1, Seq(c1,c2), s3, Seq(Seq(c5, c4), c2));
+                        assert Terminates(Seq(Seq(c5, c4), c2), s3, s2, k-1);
+                        assert typeOK(s3);
+                        var s4, k2 := Sequencing(s3, s2, Seq(c5, c4), c2, k-1);
+                        s', k' := s4, k2+1;
+                    }
+                case _ =>
+                    var (s3, c3) := TransitionSmallStep(s1, c1);
+                    assert (s3, Seq(c3, c2)) == TransitionSmallStep(s1, Seq(c1, c2));
+                    TransitionSmallStepTypeOK(s1, Seq(c1, c2), s3, Seq(c3, c2));
+                    assert Terminates(Seq(c3, c2), s3, s2, k-1);
+                    assert typeOK(s3);
+                    var s4, k2 := Sequencing(s3, s2, c3, c2, k-1);
+                    assert Terminates(c3, s3, s4, k2); 
+                    assert Terminates(c1, s1, s4, k2 + 1);
+                    s', k' := s4, k2+1;
+                    assert Terminates(c2, s4, s2, k-k'); 
+            }
+        }
+    }
 }
